LambdaGraph/Subst.lean
@@ -49,8 +49,13 @@ Variables that should remain untouched are simply mapped to themselves.
 -/
 abbrev VarMap (n : Nat) := Vector Expr n
 
+/-- Creates a new variable map of size `n` for substituting `m` with `v`. -/
+@[grind unfold]
+def VarMap.mk (n m : Nat) (v : Expr) : VarMap n :=
+  (Vector.ofFn (.var ↑·)).setIfInBounds m v
+
 /-- Updates the map to map a given variable to a variable with a fresh label. -/
-abbrev VarMap.update {n : Nat} (vm : VarMap n) (m : Nat)
+def VarMap.update {n : Nat} (vm : VarMap n) (m : Nat)
     (h : m < n := by get_elem_tactic) : VarMap (n + 1) :=
   vm.set m (.var n) |>.push (.var n)
 
@@ -76,8 +81,12 @@ distinction is necessary to support the termination proof for substitution.
 -/
 abbrev FunMap (n : Nat) := Vector (Option Nat) n
 
+/-- Creates a new function map of size `n`. -/
+@[grind unfold]
+def FunMap.mk (n : Nat) : FunMap n := Vector.ofFn (↑·)
+
 /-- Updates the map to map a given function to a function with a fresh label. -/
-abbrev FunMap.update {n : Nat} (fm : FunMap n) (m : Nat)
+def FunMap.update {n : Nat} (fm : FunMap n) (m : Nat)
     (h : m < n := by get_elem_tactic) : FunMap (n + 1) :=
   fm.set m (some n) |>.push (some n)
 
@@ -126,8 +135,7 @@ noncomputable def Expr.subst' (p : Program) (e : Expr) (vm : VarMap p.size)
           let m' := p.size
           let vm₁ := vm.update m
           let fm₁ := fm.update m
-          let dummy := (fn m').app (var m') -- temporary body that is always well-typed
-          let p₁ := p.push dummy p.ty[m]
+          let p₁ := p.push (recurse m') p.ty[m] -- temporary body that is always well-typed
           have hsize₁ : p.size ≤ p₁.size := by simp [p₁]
           have hum₁ : fm₁.unmapped < fm.unmapped := by
             simp only [FunMap.unmapped, FunMap.update, reduceCtorEq,
@@ -208,9 +216,7 @@ noncomputable def Computation.subst (p : Computation) (n : Nat) (v : Expr) :
 /-- Substitutes a value for a variable in a computation. -/
 noncomputable def Computation.subst' (p : Computation) (n : Nat) (v : Expr) :
     Computation :=
-  let vm := (Vector.ofFn fun i => .var ↑i).setIfInBounds n v
-  let fm := Vector.ofFn fun i => ↑i
-  let ⟨p', e', _, _, _⟩ := p.expr.subst' p.toProgram vm fm
+  let ⟨p', e', _, _, _⟩ := p.expr.subst' p.toProgram (.mk _ n v) (.mk _)
   ⟨p', e'⟩
 
 theorem program_subst_size_le {p : Program} {v : Expr} {n : Nat}
@@ -766,7 +772,7 @@ theorem subst_wf  {p : Program} {n : Nat} {v : Expr} {map : LabelMap p}
   intro m h
   by_cases hm : m < p.size
   · obtain ⟨-, h'⟩ := nests_of_nests_in_subst hm hp h
-    exact hwf m h'
+    exact hwf h'
   · simp only [Nat.not_lt] at hm
     have hp' : (p.subst map n v).ValidRefs := subst_validRefs hmap hp hv
     have hm' := lt_size_left_of_nests hp' h
@@ -777,14 +783,14 @@ theorem subst_wf  {p : Program} {n : Nat} {v : Expr} {map : LabelMap p}
     · have := lt_size_left_of_nestsEq hp hl
       omega
     · simp only [hmap.fwd_inj hi hj heq] at h'
-      exact hwf j h'
+      exact hwf h'
 
 theorem Program.subst_ty_eq {p : Program} {e : Expr} {vm : VarMap p.size}
     {fm : FunMap p.size} {n : Nat} (hn : n < p.size) :
     let ⟨p', _, fm', hsize, _⟩ := e.subst' p vm fm
     p'.ty[n] = p.ty[n] := by
   fun_induction Expr.subst' <;> dsimp only at *
-  next p vm fm m hm f m' vm₁ fm₁ dummy p₁ hsize₁ hum₁ p₂ f' fm₂ hsize₂ hum₂ hs₂
+  next p vm fm m hm f m' vm₁ fm₁ p₁ hsize₁ hum₁ p₂ f' fm₂ hsize₂ hum₂ hs₂
       p₃ f'' hsize hum h ih =>
     have hp₂ : p₂ = (p.fn[m].subst' p₁ vm₁ fm₁).program := by grind
     subst p₂
@@ -809,7 +815,7 @@ theorem Program.subst_fn_eq_of_lt {p : Program} {e : Expr} {vm : VarMap p.size}
   fun_induction Expr.subst' <;>
     first | grind
           | dsimp only at *
-  next p vm fm m hm f m' vm₁ fm₁ dummy p₁ hsize₁ hum₁ p₂ f' fm₂ hsize₂ hum₂ hs₂
+  next p vm fm m hm f m' vm₁ fm₁ p₁ hsize₁ hum₁ p₂ f' fm₂ hsize₂ hum₂ hs₂
       p₃ f'' hsize hum h ih =>
     have hp₂ : p₂ = (p.fn[m].subst' p₁ vm₁ fm₁).program := by grind
     subst p₂
@@ -836,12 +842,74 @@ theorem Expr.types_in_subst_of_types {p : Program} {e₁ e₂ : Expr} {t : Ty}
 
 namespace VarMap
 
+@[simp]
+theorem getElem_update_size {n : Nat} {vm : VarMap n} {m : Nat} (hm : m < n) :
+    (vm.update m hm)[n] = .var n := by simp [update]
+
+@[simp]
+theorem getElem_update_eq {n : Nat} {vm : VarMap n} {m : Nat} (hm : m < n) :
+    (vm.update m hm)[m] = .var n := by simp [update, *]
+
+@[simp]
+theorem getElem_update_ne {n : Nat} {vm : VarMap n} {m i : Nat} (hm : m < n)
+    (hi : i < n) (hne : m ≠ i) : (vm.update m hm)[i] = vm[i] := by simp [update, *]
+
+@[grind =]
+theorem getElem_update {n : Nat} {vm : VarMap n} {m i : Nat} (hm : m < n)
+    (hi : i ≤ n) :
+    (vm.update m hm)[i] = if _ : n = i ∨ m = i then .var n else vm[i] := by
+  split
+  next h =>
+    cases h
+    · simp [← ‹n = i›]
+    · simp [*]
+  next h =>
+    replace hi : i < n := by lia
+    have : m ≠ i := by simp_all
+    simp_all
+
+@[simp]
+theorem getElem_extend_lt {n n' : Nat} {vm : VarMap n} {i : Nat} (hi : i < n)
+    (hi' : i < n') : (vm.extend (n' := n'))[i] = vm[i] := by
+  simp [VarMap.extend, hi]
+
+@[simp]
+theorem getElem_extend_ge {n n' : Nat} {vm : VarMap n} {i : Nat} (hi : n ≤ i)
+    (hi' : i < n') : (vm.extend (n' := n'))[i] = .var i := by
+  replace hi : ¬i < n := by lia
+  simp [extend, hi]
+
+@[grind =]
+theorem getElem_extend {n n' : Nat} {vm : VarMap n} {i : Nat} (hi' : i < n') :
+    (vm.extend (n' := n'))[i] = if _ : i < n then vm[i] else .var i := by
+  split <;> simp_all
+
+@[simp]
+theorem extend_eq {n : Nat} {vm : VarMap n} : vm.extend (n' := n) = vm := by
+  ext i hi
+  simp [extend]
+
+theorem extend_extend {m n k : Nat} {vm : VarMap m} (h : m ≤ n) :
+    (vm.extend (n' := n) |>.extend (n' := k)) = vm.extend := by
+  ext i hi
+  by_cases i < n
+  · simp [extend, *]
+  · have : ¬i < m := by lia
+    simp [extend, *]
+
+theorem mk_types {p : Program} {n : Nat} {v : Expr} (hn : n < p.size)
+    (h : p ⊢ v : p.ty[n]) : (mk _ n v).Types p := by
+  intro m hm
+  by_cases n = m
+  · simpa [mk, *] using h
+  · simpa [mk, *] using (.var m hm)
+
 theorem update_types {p : Program} {vm : VarMap p.size} {b : Expr} {m : Nat}
     (hm : m < p.size) (h : vm.Types p) :
     (vm.update m hm).Types (p.push b p.ty[m]) := by
   intro i hi
   by_cases i = p.size
-  · simp only [Vector.getElem_push_eq, *]
+  · simp only [getElem_update_size, Vector.getElem_push_eq, *]
     have : p.ty[m] = (p.push b p.ty[m]).ty[p.size] := by simp
     conv => arg 3; rw [this]
     constructor
@@ -849,12 +917,11 @@ theorem update_types {p : Program} {vm : VarMap p.size} {b : Expr} {m : Nat}
     simp only [Vector.getElem_push_lt, hi]
     by_cases m = i
     · subst i
-      simp only [Vector.getElem_set_self]
+      simp only [getElem_update_eq]
       have : p.ty[m] = (p.push b p.ty[m]).ty[p.size] := by simp
       conv => arg 3; rw [this]
       constructor
-    · rw [Vector.getElem_set_ne _ _ ‹m ≠ i›]
-      simpa [*] using Expr.types_in_push_of_types (h i hi)
+    · simpa [*] using Expr.types_in_push_of_types (h i hi)
 
 theorem extend_types {p : Program} (e : Expr) {vm : VarMap p.size}
     (fm : FunMap p.size) (hvm : vm.Types p) :
@@ -874,25 +941,44 @@ namespace FunMap
 
 @[simp]
 theorem getElem_update_size {n : Nat} {fm : FunMap n} {m : Nat} (hm : m < n) :
-    (fm.update m hm)[n] = some n := by simp
+    (fm.update m hm)[n] = some n := by simp [update]
 
 @[simp]
 theorem getElem_update_eq {n : Nat} {fm : FunMap n} {m : Nat} (hm : m < n) :
-    (fm.update m)[m] = some n := by grind
+    (fm.update m hm)[m] = some n := by simp [update, *]
 
 @[simp]
 theorem getElem_update_ne {n : Nat} {fm : FunMap n} {m i : Nat} (hm : m < n)
-    (hi : i < n) (hne : i ≠ m) : (fm.update m hm)[i] = fm[i] := by grind
+    (hi : i < n) (hne : m ≠ i) : (fm.update m hm)[i] = fm[i] := by simp [update, *]
+
+@[grind =]
+theorem getElem_update {n : Nat} {fm : FunMap n} {m i : Nat} (hm : m < n)
+    (hi : i ≤ n) :
+    (fm.update m hm)[i] = if _ : n = i ∨ m = i then some n else fm[i] := by
+  split
+  next h =>
+    cases h
+    · simp [← ‹n = i›]
+    · simp [*]
+  next h =>
+    replace hi : i < n := by lia
+    have : m ≠ i := by simp_all
+    simp_all
+
+theorem mk_types {p : Program} : (mk _).Types p := by
+  intro m hm n heq
+  simp only [mk, Vector.getElem_ofFn, Option.some.injEq] at heq
+  simpa [heq] using hm
 
 theorem update_types {p : Program} {fm : FunMap p.size} {b : Expr} {m : Nat}
     (hm : m < p.size) (h : fm.Types p) :
     (fm.update m hm).Types (p.push b p.ty[m]) := by
   intro i hi m' heq
   by_cases i = p.size
-  · grind
+  · grind [update]
   · replace hi : i < p.size := by lia
     simp [*]
-    by_cases i = m
+    by_cases m = i
     · grind [getElem_update_eq]
     · simp only [ne_eq, not_false_eq_true, getElem_update_ne, *] at heq
       obtain ⟨_, _⟩ := h i hi _ heq
@@ -906,7 +992,7 @@ theorem subst_types {p : Program} {e : Expr} {vm : VarMap p.size}
   fun_induction Expr.subst' <;>
     first | grind
           | dsimp only at *
-  next p vm fm m hm f m' vm₁ fm₁ dummy p₁ hsize₁ hum₁ p₂ f' fm₂ hsize₂ hum₂ hs₂
+  next p vm fm m hm f m' vm₁ fm₁ p₁ hsize₁ hum₁ p₂ f' fm₂ hsize₂ hum₂ hs₂
       p₃ f'' hsize hum h ih =>
     have hp₂ : p₂ = (p.fn[m].subst' p₁ vm₁ fm₁).program := by grind
     subst p₂
@@ -917,22 +1003,19 @@ theorem subst_types {p : Program} {e : Expr} {vm : VarMap p.size}
     simp [p₁]
     by_cases i = p.size
     · subst i
-      simp only [update, fm₁] at hk
       grind
     · simp only [p₁] at hi
       replace hi : i < p.size := by lia
-      by_cases i = m
+      by_cases m = i
       · grind [getElem_update_eq]
-      · simp [fm₁, *] at hk
-        rw [getElem_update_ne _ hi ‹i ≠ m›] at hk
+      · simp only [fm₁] at hk
+        rw [getElem_update_ne _ hi ‹m ≠ i›] at hk
         obtain ⟨_, _⟩ := hfm i hi _ hk
         grind
 
 end FunMap
 
-namespace Expr
-
-theorem subst_types {p : Program} {e : Expr} {t : Ty} {vm : VarMap p.size}
+theorem Expr.subst_types {p : Program} {e : Expr} {t : Ty} {vm : VarMap p.size}
     {fm : FunMap p.size} (ht : p ⊢ e : t) (hvm : vm.Types p) (hfm : fm.Types p) :
     let ⟨p', e', _, _, _⟩ := e.subst' p vm fm
     p' ⊢ e' : t := by
@@ -944,7 +1027,7 @@ theorem subst_types {p : Program} {e : Expr} {t : Ty} {vm : VarMap p.size}
       have .var _ _ := ht
       apply hvm
     · simp [hm, ht]
-  next p vm fm m hm f m' vm₁ fm₁ dummy p₁ hsize₁ hum₁ p₂ f' fm₂ hsize₂ hum₂ hs₂
+  next p vm fm m hm f m' vm₁ fm₁ p₁ hsize₁ hum₁ p₂ f' fm₂ hsize₂ hum₂ hs₂
       p₃ f'' hsize hum h ih =>
     have .fn _ _ := ht
     have hp₂ : p₂ = (p.fn[m].subst' p₁ vm₁ fm₁).program := by grind
@@ -968,17 +1051,13 @@ theorem subst_types {p : Program} {e : Expr} {t : Ty} {vm : VarMap p.size}
     constructor <;>
       grind [types_in_subst_of_types, VarMap.extend_types, FunMap.subst_types]
 
-end Expr
-
-namespace Program
-
-theorem subst_types {p : Program} {e : Expr} {vm : VarMap p.size}
+theorem Program.subst_types {p : Program} {e : Expr} {vm : VarMap p.size}
     {fm : FunMap p.size} (ht : ⊢ p) (hvm : vm.Types p) (hfm : fm.Types p) :
     ⊢ (e.subst' p vm fm).program := by
   fun_induction Expr.subst' <;>
     first | grind [VarMap.extend_types, FunMap.subst_types]
           | dsimp only at *
-  next p vm fm m hm f m' vm₁ fm₁ dummy p₁ hsize₁ hum₁ p₂ f' fm₂ hsize₂ hum₂ hs₂
+  next p vm fm m hm f m' vm₁ fm₁ p₁ hsize₁ hum₁ p₂ f' fm₂ hsize₂ hum₂ hs₂
       p₃ f'' hsize hum h ih =>
     have ht₁ : ⊢ p₁ := by
       apply types_push ht
@@ -1006,7 +1085,794 @@ theorem subst_types {p : Program} {e : Expr} {vm : VarMap p.size}
     · rw [Vector.getElem_set_ne _ _ ‹m' ≠ i›]
       exact Expr.types_in_setBody_of_types _ (ht₂ hi)
 
-end Program
+structure FunMap.Extends {n' n : Nat} (fm' : FunMap n') (fm : FunMap n) : Prop where
+  le : n ≤ n'
+  eq : ∀ {m} (_ : m < n), fm[m].getD m ≠ m → fm'[m].getD m = fm[m].getD m
+  eq_none : ∀ {m} (_ : m < n'), fm'[m] = none → ∃ (_ : m < n), fm[m] = none
+  eq_of_lt : ∀ {m} (_ : m < n'), fm'[m].getD m < n →
+    ∃ (_ : m < n), fm'[m].getD m = fm[m].getD m
+
+grind_pattern FunMap.Extends.eq =>
+  fm'.Extends fm, fm[m].getD m, fm'[m].getD m
+
+@[grind →]
+theorem FunMap.extends_trans {n₀ n₁ n₂ : Nat} {fm₀ : FunMap n₀}
+    {fm₁ : FunMap n₁} {fm₂ : FunMap n₂} (h : fm₁.Extends fm₀)
+    (h' : fm₂.Extends fm₁) : fm₂.Extends fm₀ := by
+  obtain ⟨h₀, h₁, h₂, h₃⟩ := h
+  obtain ⟨h₀', h₁', h₂', h₃'⟩ := h'
+  constructor
+  · grind
+  · intro m hm heq₂
+    replace ⟨hm, heq₁⟩ := h₂' hm heq₂
+    exact h₂ hm heq₁
+  · grind
+  · grind
+
+theorem FunMap.extends_update {n : Nat} {fm : FunMap n} {m : Nat} (hm : m < n)
+    (h : fm[m] = none) : (fm.update m hm).Extends fm := by
+  constructor <;> grind
+
+@[grind! .]
+theorem FunMap.extends_subst {p : Program} {e : Expr} {vm : VarMap p.size}
+    {fm : FunMap p.size} : (e.subst' p vm fm).funMap.Extends fm := by
+  fun_induction Expr.subst' <;>
+    try solve | constructor <;> simp_all
+              | grind [extends_update]
+
+def Expr.NoSubst {n : Nat} (e : Expr) (fm : FunMap n) : Prop :=
+  ∀ ⦃m r⦄ (_ : m < n), e.Local (fm[m].getD m) r → fm[m].getD m = m
+
+theorem Expr.noSubst_mk {n : Nat} {e : Expr} : e.NoSubst (.mk n) := by
+  grind [Expr.NoSubst]
+
+theorem Expr.noSubst_app_iff {n : Nat} {f e : Expr} {fm : FunMap n} :
+    (f.app e).NoSubst fm ↔ f.NoSubst fm ∧ e.NoSubst fm := by
+  constructor
+  · intro h
+    and_intros
+    · intro m r hm hl
+      exact h hm (.appL _ _ _ hl)
+    · intro m r hm hl
+      exact h hm (.appR _ _ _ hl)
+  · intro ⟨hf, he⟩
+    intro m r hm hl
+    obtain hl | hl := local_app_iff.mp hl
+    · exact hf hm hl
+    · exact he hm hl
+
+theorem Expr.noSubst_cond_iff {n : Nat} {c et ef : Expr} {fm : FunMap n} :
+    (c.cond et ef).NoSubst fm ↔ c.NoSubst fm ∧ et.NoSubst fm ∧ ef.NoSubst fm := by
+  constructor
+  · intro h
+    and_intros
+    · intro m r hm hl
+      exact h hm (.condC _ _ _ _ hl)
+    · intro m r hm hl
+      exact h hm (.condT _ _ _ _ hl)
+    · intro m r hm hl
+      exact h hm (.condF _ _ _ _ hl)
+  · intro ⟨hc, het, hef⟩
+    intro m r hm hl
+    obtain hl | hl | hl := local_cond_iff.mp hl
+    · exact hc hm hl
+    · exact het hm hl
+    · exact hef hm hl
+
+theorem Expr.noSubst_of_extends_of_noSubst {n n' : Nat} {e : Expr}
+    {fm : FunMap n} {fm' : FunMap n'} (he : ∀ {m r}, e.Local m r → m < n)
+    (hext : fm'.Extends fm) (h : e.NoSubst fm) :
+    e.NoSubst fm' := by
+  intro m r hm hl
+  replace ⟨hm, heq⟩ := hext.eq_of_lt hm (he hl)
+  rw [heq] at hl ⊢
+  exact h hm hl
+
+def FunMap.LocalProvenance {n : Nat} (fm : FunMap n) (e e' : Expr) (k : Option Nat) :
+    Prop :=
+  ∀ ⦃m r⦄ (_ : m < n),
+    fm[m].getD m ≠ m → e'.Local (fm[m].getD m) r → m = k ∨ e.Local m r
+
+structure Program.ValidSubst (p : Program) (vm : VarMap p.size) (fm : FunMap p.size) where
+  validRefs : p.ValidRefs
+  vm_validRefs : ∀ {m} (_ : m < p.size), vm[m].ValidRefs p
+  vm_localProvenance : ∀ {m} (_ : m < p.size),
+    fm[m].getD m ≠ m → fm.LocalProvenance (.var m) vm[m] none
+  vm_noSubst : ∀ {m} (_ : m < p.size),
+    fm[m].getD m = m → vm[m] ≠ .var m → vm[m].NoSubst fm
+  fm_lt : ∀ {m} (_ : m < p.size), fm[m].getD m < p.size
+  fm_inj : ∀ {m n} (_ : m < p.size) (_ : n < p.size),
+    fm[m].getD m ≠ m → fm[n].getD n ≠ n → fm[m].getD m = fm[n].getD n → m = n
+  fm_idem : ∀ {m} (_ : m < p.size),
+    (fm[fm[m].getD m]'(fm_lt _)).getD (fm[m].getD m) = fm[m].getD m
+  fm_eq_none : ∀ {m n} (_ : m < p.size) (_ : n < p.size),
+    fm[m] = none → fm[n].getD n ≠ m
+  fn_localProvenance : ∀ {m} (_ : m < p.size),
+    fm[m].getD m ≠ m → fm.LocalProvenance p.fn[m] (p.fn[fm[m].getD m]'(fm_lt _)) m
+  fn_noSubst : ∀ {m} (_ : m < p.size), fm[m] = none → p.fn[m].NoSubst fm
+--  all_free_of_map_free : ∀ {m n} (_ : m < p.size) (_ : n < p.size) (_ : fm[m].getD m ≠ fm[n].getD n),
+--    (p.fn[fm[m].getD m]'(all_lt _)).Free p (fm[n].getD n) →
+--    p.fn[m].Free p n
+
+attribute [grind →] Program.ValidSubst.validRefs
+
+grind_pattern Program.ValidSubst.vm_validRefs =>
+  p.ValidSubst vm fm, m < p.size, vm[m]
+
+grind_pattern Program.ValidSubst.fm_lt =>
+  p.ValidSubst vm fm, m < p.size, fm[m].getD m
+  where m =/= Option.getD _ _
+
+theorem Program.validSubst_mk {p : Program} {n : Nat} {v : Expr}
+    (hp : p.ValidRefs) (hv : v.ValidRefs p) :
+    p.ValidSubst (.mk _ n v) (.mk _) := by
+  constructor <;> grind [Expr.NoSubst]
+
+theorem Program.validSubst_push_recurse {p : Program} {vm : VarMap p.size}
+    {fm : FunMap p.size} {i : Nat} (hi : i < p.size) (hfm : fm[i] = none)
+    (h : p.ValidSubst vm fm) :
+    (p.push (Expr.recurse p.size) p.ty[i]).ValidSubst (vm.update i hi) (fm.update i hi) := by
+  constructor
+  case validRefs =>
+    exact validRefs_push h.validRefs (by simp)
+  case vm_validRefs =>
+    intro k hk
+    by_cases k = p.size
+    · simp [*]
+    · by_cases i = k
+      · subst k
+        simp [*]
+      · replace hk : k < p.size := by lia
+        simpa [*] using Expr.validRefs_in_push (h.vm_validRefs hk)
+  case vm_localProvenance =>
+    intro m hm hmm' n r hn hnn' hl
+    have : m ≠ p.size := by
+      intro rfl
+      simp at hmm'
+    replace hm : m < p.size := by lia
+    have : n ≠ p.size := by
+      intro rfl
+      simp at hnn'
+    replace hn : n < p.size := by lia
+    by_cases i = m
+    · grind
+    · have : i ≠ n := by grind
+      apply h.vm_localProvenance <;> simp_all
+  case vm_noSubst =>
+    intro m hm hmm' hne
+    have : i ≠ m := by grind
+    have : m ≠ p.size := by
+      intro rfl
+      simp at hne
+    replace hm : m < p.size := by lia
+    simp only [ne_eq, not_false_eq_true, VarMap.getElem_update_ne, *]
+    intro n r hn hl
+    by_cases n = p.size
+    · simp [*]
+    · have : i ≠ n := by grind
+      replace hn : n < p.size := by lia
+      simp only [ne_eq, not_false_eq_true, FunMap.getElem_update_ne, *] at hl ⊢
+      refine h.vm_noSubst hm ?_ ?_ hn hl <;> simp_all
+  case fm_lt =>
+    intro k hk
+    by_cases k = p.size
+    · simp [*]
+    · replace hk : k < p.size := by lia
+      grind
+  case fm_inj =>
+    intro m n hm hn hmm' hnn' heq
+    replace hm : m < p.size := by grind
+    replace hn : n < p.size := by grind
+    have := h.fm_inj hm hn
+    grind
+  case fm_idem =>
+    intro m hm
+    by_cases m = p.size
+    · simp [*]
+    · replace hm : m < p.size := by lia
+      have := h.fm_idem hm
+      have := h.fm_eq_none hi hm hfm
+      grind
+  case fm_eq_none =>
+    intro m n hm hn heq
+    replace hm : m < p.size := by grind
+    have him : i ≠ m := by grind
+    simp only [ne_eq, not_false_eq_true, FunMap.getElem_update_ne, hm, him] at heq
+    by_cases n = p.size
+    · grind
+    · replace hn : n < p.size := by lia
+      have := h.fm_eq_none hm hn heq
+      grind
+  case fn_localProvenance =>
+    intro m hm hmm' n r hn hnn' hl
+    by_cases hnm : n = m
+    · simp [*]
+    · right
+      have : m ≠ p.size := by
+        rintro rfl
+        simp at hmm'
+      have : n ≠ p.size := by
+        rintro rfl
+        simp at hnn'
+      replace hm : m < p.size := by lia
+      replace hn : n < p.size := by lia
+      have hm' := h.fm_lt hm
+      have hn' := h.fm_lt hn
+      have him : i ≠ m := by grind
+      have hin : i ≠ n := by grind
+      simp only [ne_eq, not_false_eq_true, FunMap.getElem_update_ne, Vector.getElem_push_lt, hm,
+        him, hn, hin, hm'] at hmm' hnn' hl
+      have := h.fn_localProvenance hm hmm' hn hnn' hl
+      simp_all
+  case fn_noSubst =>
+    intro m hm heq n r hn hl
+    have : m ≠ p.size := by
+      intro rfl
+      simp at heq
+    replace hm : m < p.size := by lia
+    have : i ≠ m := by
+      intro rfl
+      simp at heq
+    simp only [Vector.getElem_push_lt, hm] at hl
+    simp only [ne_eq, not_false_eq_true, FunMap.getElem_update_ne, hm, this] at heq
+    by_cases n = p.size
+    · simp [*]
+    · replace hn : n < p.size := by lia
+      have hin : i ≠ n := by grind
+      simp only [ne_eq, not_false_eq_true, FunMap.getElem_update_ne, *] at hl ⊢
+      exact h.fn_noSubst hm heq hn hl
+
+theorem Program.validSubst_and_validRefs_and_localProvenance_subst {p : Program}
+    {e : Expr} {vm : VarMap p.size} {fm : FunMap p.size}
+    (hvalid : p.ValidSubst vm fm) (he : e.ValidRefs p) (hns : e.NoSubst fm) :
+    let ⟨p', e', fm', _, _⟩ := e.subst' p vm fm
+    p'.ValidSubst vm.extend fm' ∧ e'.ValidRefs p' ∧ fm'.LocalProvenance e e' none := by
+  fun_induction Expr.subst'
+  next p e vm fm h =>
+    simp only [VarMap.extend_eq, true_and, hvalid, he]
+    intro n r hn hnn' hl
+    right
+    simpa [hns hn hl] using hl
+  next p vm fm m h =>
+    simp only [VarMap.extend_eq, true_and, hvalid]
+    and_intros
+    · simp_all [hvalid.vm_validRefs]
+    · intro n r hn hnn' hl
+      simp only [Expr.validRefs_var_iff] at he
+      simp only [he, getElem?_pos, Option.getD_some] at hl
+      by_cases hmm' : fm[m].getD m = m
+      · simp only [Classical.not_forall] at h
+        obtain ⟨k, hk, hf, hne⟩ := h
+        have .var := hf
+        have := hvalid.vm_noSubst he hmm' hne hn hl
+        contradiction
+      · exact hvalid.vm_localProvenance he hmm' hn hnn' hl
+  next p vm fm m hm hfm m' vm₁ fm₁ p₁ hsize₁ hum₁ p₂ f' fm₂ hsize₂ hum₂ hs₂
+      p₃ f'' hsize hum h ih =>
+    rw [hs₂] at ih
+    dsimp only at ih
+    have h₁ : p₁.ValidSubst vm₁ fm₁ := validSubst_push_recurse hm hfm hvalid
+    have hns : p.fn[m].NoSubst fm₁ := by
+      intro n r hn hl
+      by_cases n = p.size
+      · simp [fm₁, *]
+      · replace hn : n < p.size := by lia
+        have hmn : m ≠ n := by grind
+        simp only [ne_eq, not_false_eq_true, FunMap.getElem_update_ne, fm₁, *] at hl ⊢
+        exact hvalid.fn_noSubst hm hfm hn hl
+    have ⟨h₂, hf', hprov⟩ :=
+      ih h₁ (Expr.validRefs_in_push (hvalid.validRefs hm)) hns
+    have hext₁ := FunMap.extends_update hm hfm
+    have hext₂ : fm₂.Extends fm₁ := by grind
+    have hext := FunMap.extends_trans hext₁ hext₂
+    and_intros
+    · constructor
+      case validRefs =>
+        exact validRefs_setBody hsize₂ h₂.validRefs hf'
+      case vm_validRefs =>
+        intro k hk
+        by_cases hk : k < p.size
+        · simp [*]
+          exact Expr.validRefs_of_size_ge (by lia) (hvalid.vm_validRefs hk)
+        · simp_all
+      case vm_localProvenance =>
+        intro k hk hkk' l r hl hll' hlc
+        by_cases k < p.size
+        · simp only [VarMap.getElem_extend_lt, *] at hlc
+          by_cases m = k
+          · subst k
+            have hl' : fm₂[l].getD l < p.size := hvalid.vm_validRefs _ hlc
+            obtain ⟨hl, heq⟩ := hext.eq_of_lt hl hl'
+            rw [heq] at hlc
+            by_cases hvmm : vm[m] = .var m
+            · grind [h₂.fm_idem]
+            · have := hvalid.vm_noSubst hm (by simp [*]) hvmm hl hlc
+              grind
+          · exact h₂.vm_localProvenance hk hkk' hl hll' (by grind)
+        · exact h₂.vm_localProvenance hk hkk' hl hll' (by grind)
+      case vm_noSubst =>
+        intro k hk hkk' hne
+        by_cases hk : k < p.size
+        · have hkk' : fm[k].getD k = k := by grind
+          simp only [VarMap.getElem_extend_lt, *] at hne ⊢
+          intro l r hl hlc
+          by_cases hll'₂ : fm₂[l].getD l = l
+          · exact hll'₂
+          · have hl' : fm₂[l].getD l < p.size := hvalid.vm_validRefs _ hlc
+            obtain ⟨hl, heq⟩ := hext.eq_of_lt hl hl'
+            rw [heq] at hlc
+            have := hvalid.vm_noSubst hk hkk' hne hl hlc
+            grind
+        · simp_all
+      case fm_lt => exact h₂.fm_lt
+      case fm_inj => exact h₂.fm_inj
+      case fm_idem => exact h₂.fm_idem
+      case fm_eq_none => exact h₂.fm_eq_none
+      case fn_localProvenance =>
+        intro n hn hnn' k r hk hkk' hl
+        have hfmm : fm₂[m].getD m = m' := by grind [hext₂.eq]
+        by_cases hnm : m = n
+        · subst n
+          simp only [Vector.getElem_set_self, p₃, hfmm] at hl
+          replace hl := hprov hk hkk' hl
+          simp only [reduceCtorEq, false_or] at hl
+          rw [hfmm] at hnn'
+          have heq : p₂.fn[m] = p.fn[m] := by
+            have hp₂ : p₂ = (p.fn[m].subst' p₁ vm₁ fm₁).program := by grind
+            subst p₂
+            rw [subst_fn_eq_of_lt (by lia)]
+            simp [p₁, hm]
+          simp [p₃, *]
+        · have hnm' : fm₂[n].getD n ≠ m' := by
+            intro heq
+            rw [← heq] at hfmm
+            have := h₂.fm_inj (by lia) hn (by lia) hnn' hfmm
+            contradiction
+          simp only [ne_eq, not_false_eq_true, Ne.symm, Vector.getElem_set_ne, p₃, hnm'] at hl
+          have hne : m' ≠ n := by grind [h₂.fm_idem]
+          cases h₂.fn_localProvenance hn hnn' hk hkk' hl <;> simp [p₃, *]
+      case fn_noSubst =>
+        intro n hn hfm' k r hk hl
+        replace ⟨hn, hfm'⟩ := hext.eq_none hn hfm'
+        have hnm' : m' ≠ n := by grind [h₂.fm_idem]
+        have heq : p₃.fn[n] = p.fn[n] := by
+          simp only [ne_eq, not_false_eq_true, Vector.getElem_set_ne, p₃, hnm']
+          have hp₂ : p₂ = (p.fn[m].subst' p₁ vm₁ fm₁).program := by grind
+          subst p₂
+          rw [subst_fn_eq_of_lt (by lia)]
+          simp [p₁, *]
+        rw [heq] at hl
+        have hk' := hvalid.validRefs hn hl
+        obtain ⟨hk, heq⟩ := hext.eq_of_lt hk hk'
+        rw [heq] at hl ⊢
+        exact hvalid.fn_noSubst hn hfm' hk hl
+    · grind
+    · intro n r hn hnn' hl
+      subst f''
+      right
+      simp only [Expr.local_fn_iff] at hl
+      obtain ⟨hr, hmn'⟩ := hl
+      have : fm₂[m].getD m = m' := by
+        rw [hext₂.eq (by lia) (by grind)]
+        simp [fm₁, m']
+      rw [← this] at hmn'
+      have : m = n := h₂.fm_inj (by lia) hn (by grind) hnn' hmn'
+      simp [*]
+  next p vm fm m hm m' hfm h =>
+    simp only [VarMap.extend_eq, Expr.validRefs_fn_iff, true_and, hvalid]
+    have hfmm : fm[m].getD m = m' := by simp [*]
+    and_intros
+    · grind
+    · intro n r hn hnn' hl
+      have hm' := hvalid.fm_lt hm
+      by_cases hmm' : m = m'
+      · have := hns hn (hmm' ▸ hl)
+        contradiction
+      · grind [hvalid.fm_inj]
+  next => grind
+  next p vm fm f e p₁ f' fm₁ hsize₁ hum₁ hs₁ p₂ e' fm₂ hsize₂ hum₂ hs₂ h ihf ihe =>
+    rw [hs₁] at ihf
+    rw [hs₂] at ihe
+    dsimp only at *
+    obtain ⟨hvf, hve⟩ := Expr.validRefs_app_iff.mp he
+    obtain ⟨hnsf, hnse⟩ := Expr.noSubst_app_iff.mp hns
+    obtain ⟨h₁, hvf', hf'⟩ := ihf hvalid hvf hnsf
+    obtain ⟨h₂, hve', he'⟩ :=
+      ihe h₁ (Expr.validRefs_of_size_ge hsize₁ hve)
+        (Expr.noSubst_of_extends_of_noSubst (by grind) (by grind) hnse)
+    and_intros
+    · grind [VarMap.extend_extend]
+    · grind [Expr.validRefs_of_size_ge]
+    · intro n r hn hnn' hl
+      have hext₁ : fm₂.Extends fm₁ := by grind
+      simp only [reduceCtorEq, Expr.local_app_iff, false_or]
+      obtain hl | hl := Expr.local_app_iff.mp hl
+      · replace ⟨hn, heq⟩ := hext₁.eq_of_lt hn (hvf' hl)
+        rw [heq] at hl
+        have := hf' hn (by grind) hl
+        grind
+      · have := he' hn hnn' hl
+        grind
+  next p vm fm b h =>
+    and_intros
+    · exact VarMap.extend_eq ▸ hvalid
+    · exact Expr.validRefs_bool
+    · intro n r hn hnn' hl
+      simp at hl
+  next p vm fm c et ef p₁ c' fm₁ hsize₁ hum₁ hs₁ vm₁ p₂ et' fm₂ hsize₂ hum₂ hs₂
+      p₃ ef' fm₃ hsize₃ hum₃ hs₃ h ihc ihet ihef =>
+    rw [hs₁] at ihc
+    rw [hs₂] at ihet
+    rw [hs₃] at ihef
+    dsimp only at *
+    obtain ⟨hvc, hvet, hvef⟩ := Expr.validRefs_cond_iff.mp he
+    obtain ⟨hnsc, hnset, hnsef⟩ := Expr.noSubst_cond_iff.mp hns
+    obtain ⟨h₁, hvc', hc'⟩ := ihc hvalid hvc hnsc
+    obtain ⟨h₂, hvet', het'⟩ :=
+      ihet h₁ (Expr.validRefs_of_size_ge hsize₁ hvet)
+        (Expr.noSubst_of_extends_of_noSubst (by grind) (by grind) hnset)
+    obtain ⟨h₃, hvef', hef'⟩ :=
+      ihef h₂ (Expr.validRefs_of_size_ge (by lia) hvef)
+        (Expr.noSubst_of_extends_of_noSubst (by grind) (by grind) hnsef)
+    and_intros
+    · grind [VarMap.extend_extend]
+    · grind [Expr.validRefs_of_size_ge]
+    · intro n r hn hnn' hl
+      have hext₁ : fm₃.Extends fm₁ := by grind
+      have hext₂ : fm₃.Extends fm₂ := by grind
+      simp only [reduceCtorEq, Expr.local_cond_iff, false_or]
+      obtain hl | hl | hl := Expr.local_cond_iff.mp hl
+      · replace ⟨hn, heq⟩ := hext₁.eq_of_lt hn (hvc' hl)
+        rw [heq] at hl
+        have := hc' hn (by grind) hl
+        grind
+      · replace ⟨hn, heq⟩ := hext₂.eq_of_lt hn (hvet' hl)
+        rw [heq] at hl
+        have := het' hn (by grind) hl
+        grind
+      · have := hef' hn hnn' hl
+        grind
+
+theorem Program.validSubst_subst {p : Program} {e : Expr} {vm : VarMap p.size}
+    {fm : FunMap p.size} (hvalid : p.ValidSubst vm fm) (he : e.ValidRefs p)
+    (hns : e.NoSubst fm) :
+    let ⟨p', _, fm', _, _⟩ := e.subst' p vm fm
+    p'.ValidSubst vm.extend fm' :=
+  Program.validSubst_and_validRefs_and_localProvenance_subst hvalid he hns |>.1
+
+theorem Expr.validRefs_subst {p : Program} {e : Expr} {vm : VarMap p.size}
+    {fm : FunMap p.size} (hvalid : p.ValidSubst vm fm) (he : e.ValidRefs p)
+    (hns : e.NoSubst fm) :
+    let ⟨p', e', _, _, _⟩ := e.subst' p vm fm
+    e'.ValidRefs p' :=
+  Program.validSubst_and_validRefs_and_localProvenance_subst hvalid he hns |>.2.1
+
+theorem Expr.localProvenance_subst {p : Program} {e : Expr} {vm : VarMap p.size}
+    {fm : FunMap p.size} (hvalid : p.ValidSubst vm fm) (he : e.ValidRefs p)
+    (hns : e.NoSubst fm) :
+    let ⟨_, e', fm', _, _⟩ := e.subst' p vm fm
+    fm'.LocalProvenance e e' none :=
+  Program.validSubst_and_validRefs_and_localProvenance_subst hvalid he hns |>.2.2
+
+theorem Program.exists_of_ge_in_subst {p : Program} {e : Expr}
+    {vm : VarMap p.size} {fm : FunMap p.size} (h : p.ValidSubst vm fm)
+    (he : e.ValidRefs p) (hns : e.NoSubst fm) {n' : Nat} (hn' : p.size ≤ n') :
+    let ⟨p', _, fm', _, _⟩ := e.subst' p vm fm
+    n' < p'.size → ∃ (n : Nat) (_ : n < p.size), n' = fm'[n].getD n := by
+  intro hlt
+  fun_induction Expr.subst' generalizing n' <;> try grind
+  next p vm fm m hm hfm m' vm₁ fm₁ p₁ hsize₁ hum₁ p₂ f' fm₂ hsize₂ hum₂ hs₂
+      p₃ f'' hsize hum h ih =>
+    rw [hs₂] at ih
+    dsimp only at *
+    have hext : fm₂.Extends fm₁ := by grind
+    have hfm' : fm₂[m].getD m = p.size := by
+      rw [hext.eq (by lia) (by grind)]
+      simp [fm₁]
+    have h₁ : p₁.ValidSubst vm₁ fm₁ := validSubst_push_recurse hm hfm h
+    have hns : p.fn[m].NoSubst fm₁ := by
+      intro n r hn hl
+      by_cases n = p.size
+      · simp [fm₁, *]
+      · replace hn : n < p.size := by lia
+        have hmn : m ≠ n := by grind
+        simp only [ne_eq, not_false_eq_true, FunMap.getElem_update_ne, fm₁, *] at hl ⊢
+        exact h.fn_noSubst hm hfm hn hl
+    have h₂ : p₂.ValidSubst vm₁.extend fm₂ := by
+      have hp₂ : p₂ = (p.fn[m].subst' p₁ vm₁ fm₁).program := by grind
+      subst p₂
+      have hfm₂ : fm₂ = (p.fn[m].subst' p₁ vm₁ fm₁).funMap := by grind
+      subst fm₂
+      exact validSubst_subst h₁ (Expr.validRefs_in_push (h.validRefs hm)) hns
+    by_cases n' = p.size
+    · refine ⟨m, hm, ?_⟩
+      rwa [hfm']
+    · obtain ⟨n, hn, heq⟩ :=
+        ih (validSubst_push_recurse hm hfm h)
+          (Expr.validRefs_in_push (h.validRefs hm)) hns (by lia) hlt
+      have : n ≠ p.size := by grind [h₂.fm_idem]
+      exact ⟨n, by lia, heq⟩
+  next p vm fm f e p₁ f' fm₁ hsize₁ hum₁ hs₁ p₂ e' fm₂ hsize₂ hum₂ hs₂ h ihf ihe =>
+    rw [hs₁] at ihf
+    rw [hs₂] at ihe
+    dsimp only at *
+    obtain ⟨hvf, hve⟩ := Expr.validRefs_app_iff.mp he
+    obtain ⟨hnsf, hnse⟩ := Expr.noSubst_app_iff.mp hns
+    have h₁ : p₁.ValidSubst vm.extend fm₁ := by
+      grind [validSubst_subst]
+    have h₂ : p₂.ValidSubst vm.extend fm₂ := by
+      grind [validSubst_subst, VarMap.extend_extend, Expr.validRefs_of_size_ge,
+        Expr.noSubst_of_extends_of_noSubst]
+    have hext₁ : fm₂.Extends fm₁ := by grind
+    by_cases n' < p₁.size
+    · grind
+    · replace hn' : p₁.size ≤ n' := by lia
+      obtain ⟨n, hlt, heq⟩ := ihe h₁ (Expr.validRefs_of_size_ge hsize₁ hve)
+        (Expr.noSubst_of_extends_of_noSubst (by grind) (by grind) hnse) hn' hlt
+      by_cases hn : n < p.size
+      · exact ⟨n, hn, heq⟩
+      · grind [h₂.fm_idem]
+  next p vm fm c et ef p₁ c' fm₁ hsize₁ hum₁ hs₁ vm₁ p₂ et' fm₂ hsize₂ hum₂ hs₂
+      p₃ ef' fm₃ hsize₃ hum₃ hs₃ h ihc ihet ihef =>
+    rw [hs₁] at ihc
+    rw [hs₂] at ihet
+    rw [hs₃] at ihef
+    dsimp only at *
+    obtain ⟨hvc, hvet, hvef⟩ := Expr.validRefs_cond_iff.mp he
+    obtain ⟨hnsc, hnset, hnsef⟩ := Expr.noSubst_cond_iff.mp hns
+    have h₁ : p₁.ValidSubst vm₁ fm₁ := by
+      grind [validSubst_subst]
+    have h₂ : p₂.ValidSubst vm₁.extend fm₂ := by
+      grind [validSubst_subst, VarMap.extend_extend, Expr.validRefs_of_size_ge,
+        Expr.noSubst_of_extends_of_noSubst]
+    have h₃ : p₃.ValidSubst vm₁.extend fm₃ := by
+      grind [validSubst_subst, VarMap.extend_extend, Expr.validRefs_of_size_ge,
+        Expr.noSubst_of_extends_of_noSubst]
+    have hext₁₂ : fm₂.Extends fm₁ := by grind
+    have hext₁₃ : fm₃.Extends fm₁ := by grind
+    have hext₂₃ : fm₃.Extends fm₂ := by grind
+    by_cases n' < p₁.size
+    · obtain ⟨n, hlt, heq⟩ := ihc h hvc hnsc hn' ‹_›
+      grind
+    · replace hn' : p₁.size ≤ n' := by lia
+      by_cases n' < p₂.size
+      · obtain ⟨n, hlt, heq⟩ := ihet h₁ (Expr.validRefs_of_size_ge hsize₁ hvet)
+          (Expr.noSubst_of_extends_of_noSubst (by grind) (by grind) hnset) hn' ‹_›
+        by_cases hn : n < p.size
+        · grind
+        · replace hn : p.size ≤ n := by lia
+          obtain ⟨m, hlt', heq'⟩ := ihc h hvc hnsc hn hlt
+          have := hext₁₂.eq (show m < p₁.size by lia) (by lia)
+          grind [h₂.fm_idem]
+      · replace hn' : p₂.size ≤ n' := by lia
+        obtain ⟨n, hlt, heq⟩ := ihef h₂ (Expr.validRefs_of_size_ge (by lia) hvef)
+          (Expr.noSubst_of_extends_of_noSubst (by grind) (by grind) hnsef) hn' hlt
+        by_cases hn : n < p.size
+        · exact ⟨n, hn, heq⟩
+        · replace hn : p.size ≤ n := by lia
+          by_cases n < p₁.size
+          · obtain ⟨m, hlt', heq'⟩ := ihc h hvc hnsc hn ‹_›
+            have := hext₁₂.eq (show m < p₁.size by lia) (by lia)
+            grind [h₃.fm_idem]
+          · replace hn : p₁.size ≤ n := by lia
+            obtain ⟨m, hlt', heq'⟩ := ihet h₁ (Expr.validRefs_of_size_ge hsize₁ hvet)
+              (Expr.noSubst_of_extends_of_noSubst (by grind) (by grind) hnset) hn ‹_›
+            have := hext₂₃.eq (show m < p₂.size by lia) (by lia)
+            grind [h₃.fm_idem]
+
+theorem Program.lt_size_of_pathWithout_of_lt {p : Program} {e : Expr}
+    {vm : VarMap p.size} {fm : FunMap p.size} (hp : p.ValidRefs) {m n k : Nat}
+    (hm : m < p.size) (hp : m ⟶[(e.subst' p vm fm).program, n]* k) :
+    k < p.size := by
+  induction hp with
+  | refl m hm => exact hm
+  | step m l k hne hs hp ih =>
+    obtain ⟨_, hlf⟩ := hs
+    rw [subst_fn_eq_of_lt hm] at hlf
+    grind
+
+theorem Program.pathWithout_of_pathWithout_in_subst {p : Program} {e : Expr}
+    {vm : VarMap p.size} {fm : FunMap p.size} (h : p.ValidSubst vm fm)
+    (he : e.ValidRefs p) (hns : e.NoSubst fm) {n' m' k' : Nat} (hn' : p.size ≤ n')
+    (hm' : p.size ≤ m') (hk' : p.size ≤ k') :
+    let ⟨p', _, fm', _, _⟩ := e.subst' p vm fm
+    n' < p'.size → m' < p'.size → k' < p'.size → m' ⟶[p', n']* k' →
+      ∃ (n m k : Nat) (hn : n < p.size) (hm : m < p.size) (hk : k < p.size),
+        n' = fm'[n].getD n ∧ m' = fm'[m].getD m ∧ k' = fm'[k].getD k ∧ m ⟶[p, n]* k := by
+  intro hnlt hmlt hklt hp'
+  let p' := (e.subst' p vm fm).program
+  let e' := (e.subst' p vm fm).expr
+  let fm' := (e.subst' p vm fm).funMap
+  have hsize := (e.subst' p vm fm).size_ge
+  have h' : p'.ValidSubst vm.extend fm' := Program.validSubst_subst h he hns
+  induction hp' with
+  | refl m' hne' =>
+    obtain ⟨n, hn, hfmn⟩ := exists_of_ge_in_subst h he hns hn' hnlt
+    obtain ⟨k, hk, hfmk⟩ := exists_of_ge_in_subst h he hns hk' hklt
+    obtain ⟨m, hm, hfmm⟩ := exists_of_ge_in_subst h he hns hm' hmlt
+    have hne : n ≠ m := by grind
+    exact ⟨n, m, m, hn, hm, hm, hfmn, hfmm, hfmm, .refl _ hne⟩
+  | step m' l' k' hne' hs' hp' ih =>
+    obtain ⟨m, hm, hfmm⟩ := exists_of_ge_in_subst h he hns hm' hmlt
+    have hl' : p.size ≤ l' := by
+      false_or_by_contra
+      rename_i hl'
+      have := lt_size_of_pathWithout_of_lt h.validRefs (by simpa using hl') hp'
+      lia
+    obtain ⟨_, hlf'⟩ := hs'
+    have hllt : l' < p'.size := by grind
+    have ⟨n, l, k, hn, hl, hk, hfmn, hfml, hfmk, hp⟩ := ih hl' hk' hllt hklt
+    have hne : n ≠ m := by grind
+    have hlf := h'.fn_localProvenance
+      (show m < p'.size by lia) (by lia) (show l < p'.size by lia) (by lia)
+      (by simpa [*] using hlf')
+    simp only [Option.some.injEq, Program.subst_fn_eq_of_lt hm, p'] at hlf
+    obtain heq | hlf := hlf
+    · grind
+    · refine ⟨n, m, k, hn, hm, hk, hfmn, hfmm, hfmk, .step _ _ _ hne ⟨hm, hlf⟩ hp⟩
+
+theorem Program.free_in_fn_of_free_in_subst_of_ge {p : Program} {e : Expr}
+    {vm : VarMap p.size} {fm : FunMap p.size} (h : p.ValidSubst vm fm)
+    (he : e.ValidRefs p) (hns : e.NoSubst fm) {n' m' : Nat} (hn' : p.size ≤ n')
+    (hm' : p.size ≤ m') (hne' : n' ≠ m') :
+    let ⟨p', _, fm', _, _⟩ := e.subst' p vm fm
+    ∀ (_ : m' < p'.size), p'.fn[m'].Free p' n' →
+      ∃ (n m : Nat) (hn : n < p.size) (hm : m < p.size),
+        n' = fm'[n].getD n ∧ m' = fm'[m].getD m ∧ p.fn[m].Free p n := by
+  intro hmlt hf'
+  let p' := (e.subst' p vm fm).program
+  let e' := (e.subst' p vm fm).expr
+  let fm' := (e.subst' p vm fm).funMap
+  have h' : p'.ValidSubst vm.extend fm' := Program.validSubst_subst h he hns
+  obtain ⟨k', hklt, hlv', hp'⟩ := (free_in_fn_iff hmlt hne').mp hf'
+  have hk' : p.size ≤ k' := by grind [subst_fn_eq_of_lt]
+  have hnlt : n' < p'.size := by grind
+  obtain ⟨n, m, k, hn, hm, hk, hfmn, hfmm, hfmk, hp⟩ :=
+    pathWithout_of_pathWithout_in_subst h he hns hn' hm' hk' hnlt hmlt hklt hp'
+  have hne : n ≠ m := by grind
+  have hlv := h'.fn_localProvenance
+    (show k < p'.size by lia) (by lia) (show n < p'.size by lia) (by lia)
+    (by simpa [hfmn, hfmk] using hlv')
+  rw [subst_fn_eq_of_lt hk] at hlv
+  simp only [Option.some.injEq, hp.ne_end, false_or] at hlv
+  exact ⟨n, m, hn, hm, hfmn, hfmm, (free_in_fn_iff hm hne).mpr ⟨k, hk, hlv, hp⟩⟩
+
+theorem Expr.free_of_free_in_subst_of_ge {p : Program} {e : Expr}
+    {vm : VarMap p.size} {fm : FunMap p.size} (h : p.ValidSubst vm fm)
+    (he : e.ValidRefs p) (hns : e.NoSubst fm) {n' : Nat} (hn' : p.size ≤ n') :
+    let ⟨p', e', fm', _, _⟩ := e.subst' p vm fm
+    e'.Free p' n' → ∃ (n : Nat) (_ : n < p.size),
+      n' = fm'[n].getD n ∧ e.Free p n := by
+  intro hf
+  let p' := (e.subst' p vm fm).program
+  let e' := (e.subst' p vm fm).expr
+  let fm' := (e.subst' p vm fm).funMap
+  have h' : p'.ValidSubst vm.extend fm' := Program.validSubst_subst h he hns
+  have hlt : n' < p'.size :=
+    lt_size_of_free h'.validRefs (validRefs_subst h he hns) hf
+  obtain ⟨n, hn, heq⟩ := Program.exists_of_ge_in_subst h he hns hn' hlt
+  obtain hlv' | ⟨m', k', hk', hlf', hp', hlv'⟩ := free_iff.mp hf
+  · refine ⟨n, hn, heq, free_of_localVar ?_⟩
+    simpa using localProvenance_subst h he hns (by lia) (by lia) (heq ▸ hlv')
+  · by_cases hm' : m' < p.size
+    · replace hk' := Program.lt_size_of_pathWithout_of_lt h.validRefs ‹_› hp'
+      grind [Program.subst_fn_eq_of_lt]
+    · simp only [Nat.not_lt] at hm'
+      have hk' : p.size ≤ k' := by grind [Program.subst_fn_eq_of_lt]
+      obtain ⟨n, m, k, hn, hm, hk, hfmn, hfmm, hfmk, hp⟩ :=
+        Program.pathWithout_of_pathWithout_in_subst h he hns hn' hm' hk'
+          ‹_› (validRefs_subst h he hns hlf') ‹_› hp'
+      have hlf := localProvenance_subst h he hns
+        (show m < p'.size by lia) (by lia) (by simpa [*] using hlf')
+      simp only [reduceCtorEq, false_or] at hlf
+      have hlv := h'.fn_localProvenance
+        (show k < p'.size by lia) (by lia) (show n < p'.size by lia) (by lia)
+        (by simpa [hfmn, hfmk] using hlv')
+      rw [Program.subst_fn_eq_of_lt hk] at hlv
+      simp only [Option.some.injEq, hp.ne_end, false_or] at hlv
+      exact ⟨n, hn, hfmn, free_iff.mpr <| Or.inr ⟨m, k, hk, hlf, hp, hlv⟩⟩
+
+theorem Program.lt_size_of_free_in_subst_of_lt {p : Program} {e : Expr}
+    {vm : VarMap p.size} {fm : FunMap p.size} (h : p.ValidRefs)
+    {n m : Nat} (hm : m < p.size) (hne : n ≠ m) :
+    let ⟨p', _, _, _, _⟩ := e.subst' p vm fm
+    p'.fn[m].Free p' n → n < p.size := by
+  intro hf
+  obtain ⟨k, hk, hlv, hp⟩ := (free_in_fn_iff (by lia) hne).mp hf
+  have hk := lt_size_of_pathWithout_of_lt h hm hp
+  rw [subst_fn_eq_of_lt hk] at hlv
+  exact h hk hlv
+
+theorem Program.lt_size_of_nests_in_subst_of_lt {p : Program} {e : Expr}
+    {vm : VarMap p.size} {fm : FunMap p.size} (h : p.ValidRefs) {n m : Nat}
+    (hm : m < p.size) (hnests : n ≻[(e.subst' p vm fm).program] m) :
+    n < p.size := by
+  induction hnests with
+  | free m hm' hne hf =>
+    exact lt_size_of_free_in_subst_of_lt h hm hne hf
+  | step k m hm hne hf hnests ih =>
+    exact ih <| lt_size_of_free_in_subst_of_lt h hm hne hf
+
+theorem Expr.validRefs_in_subst {p : Program} {e₁ e₂ : Expr}
+    {vm : VarMap p.size} {fm : FunMap p.size} (he₁ : e₁.ValidRefs p) :
+    e₁.ValidRefs (e₂.subst' p vm fm).program :=
+  let ⟨_, _, _, hsize, _⟩ := (e₂.subst' p vm fm)
+  validRefs_of_size_ge hsize he₁
+
+theorem Expr.free_of_free_in_subst {p : Program} {e₁ e₂ : Expr}
+    {vm : VarMap p.size} {fm : FunMap p.size} {n : Nat} (hp : p.ValidRefs)
+    (he₁ : e₁.ValidRefs p) (hf : e₁.Free (e₂.subst' p vm fm).program n) :
+    e₁.Free p n := by
+  generalize hp' : (e₂.subst' p vm fm).program = p' at hf
+  induction hf with
+    try grind [Free.var, Free.appL, Free.appR, Free.condC, Free.condT, Free.condF]
+  | fn k hk' hne hf ih =>
+    simp only [validRefs_fn_iff] at he₁
+    constructor
+    · exact hne
+    · subst p'
+      rw [Program.subst_fn_eq_of_lt he₁] at ih
+      exact ih (hp he₁)
+
+theorem Program.nests_of_nests_in_subst_of_lt {p : Program} {e : Expr}
+    {vm : VarMap p.size} {fm : FunMap p.size} {m n : Nat} (hn : n < p.size)
+    (hp : p.ValidRefs) (h : m ≻[(e.subst' p vm fm).program] n) :
+    m ≻[p] n := by
+  generalize hp' : (e.subst' p vm fm).program = p' at h
+  induction h with
+  | free n hn' hne hf' =>
+    subst p'
+    have hf : p.fn[n].Free p m := by
+      apply Expr.free_of_free_in_subst hp (hp hn)
+      simpa [subst_fn_eq_of_lt hn] using hf'
+    exact Nests.free _ hn hne hf
+  | step k n hn' hne hf' h ih =>
+    subst p'
+    have hf : p.fn[n].Free p k := by
+      apply Expr.free_of_free_in_subst hp (hp hn)
+      simpa [subst_fn_eq_of_lt hn] using hf'
+    exact Nests.step _ _ hn hne hf (ih (lt_size_of_free hp (hp hn) hf))
+
+theorem Program.nests_of_nests_in_subst_of_ge {p : Program} {e : Expr}
+    {vm : VarMap p.size} {fm : FunMap p.size} (h : p.ValidSubst vm fm)
+    (he : e.ValidRefs p) (hns : e.NoSubst fm) {n' m' : Nat} (hn' : p.size ≤ n') :
+    let ⟨p', _, fm', _, _⟩ := e.subst' p vm fm
+    n' ≻[p'] m' → ∃ (n m : Nat) (hn : n < p.size) (hm : m < p.size),
+      n' = fm'[n].getD n ∧ m' = fm'[m].getD m ∧ n ≻[p] m := by
+  intro hnests'
+  let p' := (e.subst' p vm fm).program
+  let e' := (e.subst' p vm fm).expr
+  let fm' := (e.subst' p vm fm).funMap
+  have h' : p'.ValidSubst vm.extend fm' := Program.validSubst_subst h he hns
+  induction hnests' with
+  | free m' hltm hne' hf' =>
+    have hm' : p.size ≤ m' := by
+      false_or_by_contra
+      rename_i hm'
+      simp only [Nat.not_le] at hm'
+      have := lt_size_of_free_in_subst_of_lt h.validRefs hm' hne' hf'
+      lia
+    obtain ⟨n, m, hn, hm, hfmn, hfmm, hf⟩ :=
+      Program.free_in_fn_of_free_in_subst_of_ge h he hns hn' hm' hne' hltm hf'
+    have hne : n ≠ m := by grind
+    exact ⟨n, m, hn, hm, hfmn, hfmm, .free _ hm hne hf⟩
+  | step k' m' hmlt hne' hf' hnests' ih =>
+    obtain ⟨n, k, hn, hk, hfmn, hfmk, hnests⟩ := ih
+    have hk' : p.size ≤ k' := by
+      false_or_by_contra
+      rename_i hk'
+      have := lt_size_of_nests_in_subst_of_lt h.validRefs (by simpa using hk') hnests'
+      lia
+    have hm' : p.size ≤ m' := by
+      false_or_by_contra
+      rename_i hm'
+      have := lt_size_of_free_in_subst_of_lt h.validRefs (by simpa using hm') hne' hf'
+      lia
+    obtain ⟨l, m, hl, hm, hfml, hfmm, hf⟩ :=
+      free_in_fn_of_free_in_subst_of_ge h he hns hk' hm' hne' hmlt hf'
+    obtain rfl : k = l := h'.fm_inj (by lia) (by lia) (by lia) (by lia) (hfmk ▸ hfml)
+    have hne : k ≠ m := by grind
+    exact ⟨n, m, hn, hm, hfmn, hfmm, .step _ _ hm hne hf hnests⟩
 
 namespace Computation
 
@@ -1015,12 +1881,23 @@ theorem subst_types {c : Computation} {t : Ty} {n : Nat} {v : Expr}
     ⊢ c.subst' n v : t := by
   refine ⟨Program.subst_types ht.program_types ?hvm ?hfm,
           Expr.subst_types ht.expr_types ?hvm ?hfm⟩
-  · intro i hi
-    by_cases n = i
-    · simp_all
-    · rw [Vector.getElem_setIfInBounds_ne _ ‹n ≠ i›, Vector.getElem_ofFn]
-      constructor
-  · intro i hi m heq
-    grind
+  · exact VarMap.mk_types hn hv
+  · exact FunMap.mk_types
+
+theorem subst_wf {c : Computation} {n : Nat} {v : Expr} (hp : c.ValidRefs)
+    (he : c.expr.ValidRefs c.toProgram) (hv : v.ValidRefs c.toProgram)
+    (h : c.WF) : (c.subst' n v).WF := by
+  let ⟨p, e⟩ := c
+  dsimp only [subst'] at *
+  intro m hnests
+  by_cases hm : m < p.size
+  · exact h <| Program.nests_of_nests_in_subst_of_lt hm hp hnests
+  · simp only [Nat.not_lt] at hm
+    have hvalid := Program.validSubst_mk (n := n) hp hv
+    have hvalid' := Program.validSubst_subst hvalid he Expr.noSubst_mk
+    replace ⟨k, l, hk, hl, hfmk, hfml, hnests⟩ :=
+      Program.nests_of_nests_in_subst_of_ge hvalid he Expr.noSubst_mk hm hnests
+    obtain rfl : k = l := hvalid'.fm_inj (by lia) (by lia) (by lia) (by lia) (hfmk ▸ hfml)
+    exact h hnests
 
 end Computation
